theories/switcher/switcher_helpers.v
@@ -26,48 +26,6 @@ Section switcher_helper.
   Implicit Types W : WORLD.
   Implicit Types C : CmptName.
 
-  (* TODO Move the lemmas into a helper file for switcher spec *)
-
-  (* TODO the following seems like it's always used in sequence with
-    [decompose_opening_to_closing_resources],
-    so maybe they should be put together somehow!! *)
-  Lemma open_world_interp_opening_resources (W : WORLD) (C : CmptName)
-    (la la' : list Addr) (g : Locality) (b e a : Addr) :
-    NoDup la ->
-    Forall (fun a' : Addr => (b <= a' < e)%a ) la ->
-    la ## la' ->
-
-    interp W C (WCap RWL g b e a)
-    ∗ world_interp_open W C la'
-      -∗
-
-    world_interp_open W C (la++la')
-    ∗ ([∗ list] a ∈ la, opening_resources interp W C a)
-  .
-  Proof.
-    rewrite world_interp_open_eq /world_interp_open_def.
-    iIntros (???) "(#Hinterp & [Hr Hsts] )"; cbn in * |- *.
-    iDestruct (region_open_list_interp_gen _ _ _ _
-                with "[$Hinterp $Hr $Hsts]") as "[$ $]"; eauto.
-  Qed.
-
-  Lemma close_world_interp_opening_resources (W : WORLD) (C : CmptName)
-  (lv : list Word)
-  (la la' : list Addr):
-
-    NoDup la ->
-    la ## la' ->
-    length lv = length la ->
-
-    world_interp_open W C (la++la')
-    ∗ ([∗ list] a ; v ∈ la ; lv, a ↦ₐ v ∗ closing_resources interp W C a v)
-    -∗ world_interp_open W C la'.
-  Proof.
-    rewrite world_interp_open_eq /world_interp_open_def.
-    iIntros (???) "([Hr Hsts] & Hres )"; cbn in * |- *.
-    iDestruct (region_close_list_interp_gen with "[$Hres $Hr]") as "$"; eauto.
-  Qed.
-
   Lemma world_interp_reinstate_stack  E W C la lv :
     NoDup la →
     Forall (eq (WInt 0)) lv ->
@@ -102,7 +60,14 @@ Section switcher_helper.
     rewrite world_interp_eq /world_interp_def /revoked_addresses.
     iIntros (Hdup) "(Hl & [Hr Hsts] )".
     iMod ( monotone_revoke_keep _ _ l with "[$Hr $Hsts Hl]") as
-      "($ & $ & ? & $)"; auto.
+      "($ & $ & Hres & $)"; auto.
+    rewrite /RevokedResources.
+    iModIntro; iNext.
+    iApply (big_sepL_impl with "Hres").
+    iModIntro; iIntros (k ka Hka) "(%pa & %Pa & %Hpers_Pa & Htmp_res & Hrel)".
+    iDestruct "Htmp_res" as "(%va & Hpa_O & Ha & Hmono & HPa)".
+    iFrame "∗%".
+    by rewrite mono_temporary_eq.
   Qed.
 
   (* TODO This theorem is essentially [reinstate_world], but with different RevokedResources *)
@@ -118,6 +83,7 @@ Section switcher_helper.
     done.
   Qed.
 
+  (* TODO understand how [close_list_resources_gen] is being used! *)
   (* TODO USED IN INTERP RETURN *)
   Lemma open_world_interp_cframe
     (W : WORLD) (C : CmptName) (b_stk e_stk a_stk a_stk4 : Addr)
@@ -144,7 +110,7 @@ Section switcher_helper.
       let la := (if (is_untrusted_caller ccrel) then finz.seq_between a_stk (a_stk ^+ 4)%a else []) in
       let lv := (if (is_untrusted_caller ccrel) then [wastk;wastk1;wastk2;wastk3] else []) in
       ([[ a_stk , (a_stk ^+ 4)%a ]] ↦ₐ [[ [wastk;wastk1;wastk2;wastk3] ]])
-      ∗ ▷ ([∗ list] a ; v ∈ la ; lv, ▷ closing_resources interp W C a v)
+      ∗ ▷ StackWorldResources interp W C la lv
       ∗ (⌜if (is_untrusted_caller ccrel)
          then True
          else (wastk = wcs2 ∧ wastk1 = wcs3 ∧ wastk2 = wret ∧ wastk3 = wcgp0)⌝)
@@ -156,6 +122,7 @@ Section switcher_helper.
     destruct (is_untrusted_caller ccrel); cycle 1.
     * iExists wcs2, wcs3, wret, wcgp0.
       iEval (rewrite -open_world_interp_empty) in "Hworld_interp"; iFrame "Hworld_interp".
+      rewrite /StackWorldResources.
       iSplitL "Hcframe_interp"; auto.
       iDestruct "Hcframe_interp" as "(?&?&?&?)".
       iApply (region_pointsto_cons _ (a_stk ^+ 1)%a); [solve_addr+Ha_stk4|solve_addr+He_a1|]; iFrame.
@@ -177,40 +144,28 @@ Section switcher_helper.
       cbn.
       replace ((a_stk ^+ 1) ^+ 1)%a with (a_stk ^+ 2)%a by solve_addr+Ha_stk4.
       replace ((a_stk ^+ 2) ^+ 1)%a with (a_stk ^+ 3)%a by solve_addr+Ha_stk4.
-      cbn.
-      iDestruct "Hres" as "(Hres0 & Hres1 & Hres2 & Hres3 & _)".
-      iDestruct (opening_closing_resources with "Hres0") as (wastk) "[Hres0 Ha0]".
-      iDestruct (opening_closing_resources with "Hres1") as (wastk1) "[Hres1 Ha1]".
-      iDestruct (opening_closing_resources with "Hres2") as (wastk2) "[Hres2 Ha2]".
-      iDestruct (opening_closing_resources with "Hres3") as (wastk3) "[Hres3 Ha3]".
       iFrame.
-      iApply (region_pointsto_cons _ (a_stk ^+ 1)%a); [solve_addr+Ha_stk4|solve_addr+He_a1|]; iFrame.
-      iApply (region_pointsto_cons _ (a_stk ^+ 2)%a); [solve_addr+Ha_stk4|solve_addr+He_a1|]; iFrame.
-      iApply (region_pointsto_cons _ (a_stk ^+ 3)%a); [solve_addr+Ha_stk4|solve_addr+He_a1|]; iFrame.
-      iApply (region_pointsto_cons _ (a_stk ^+ 4)%a); [solve_addr+Ha_stk4|solve_addr+He_a1|]; iFrame.
-      by rewrite /region_pointsto finz_seq_between_empty.
+      iDestruct "Hres" as "(%lv & [Hlv Hres])".
+      iDestruct (big_sepL2_length with "Hlv") as "%Hlv_len".
+      repeat (destruct lv; try done).
+      iExists w, w0, w1, w2.
+      iFrame.
+      iSplitL "Hlv".
+      - replace ( [a_stk; (a_stk ^+ 1)%a; (a_stk ^+ 2)%a; (a_stk ^+ 3)%a] )
+        with (finz.seq_between a_stk (a_stk ^+4)%a); first done.
+        repeat (rewrite finz_seq_between_cons; last solve_addr+He_a1).
+        replace ( ((a_stk ^+ 1) ^+ 1)%a ) with ((a_stk ^+ 2))%a by solve_addr+He_a1.
+        replace ( ((a_stk ^+ 2) ^+ 1)%a ) with ((a_stk ^+ 3))%a by solve_addr+He_a1.
+        replace ( ((a_stk ^+ 3) ^+ 1)%a ) with ((a_stk ^+ 4))%a by solve_addr+He_a1.
+        rewrite finz_seq_between_empty; last solve_addr+He_a1.
+        done.
+      - iNext. rewrite /StackWorldResources.
+        repeat (iDestruct (big_sepL2_cons with "Hres") as "[$ Hres]").
   Qed.
 
-  Lemma decompose_opening_to_closing_resources W C la :
-    ([∗ list] a ∈ la, opening_resources interp W C a) -∗
-    (∃ (lv : list Word),
-        ⌜ length lv = length la ⌝
-        ∗ ▷ ([∗ list] a ; v ∈ la; lv, closing_resources interp W C a v)
-        ∗ ([∗ list] a ; v ∈  la ; lv, a ↦ₐ v)
-    ).
-  Proof.
-    induction la; cbn; iIntros "Hres".
-    - iExists []; cbn; done.
-    - iDestruct "Hres" as "[Ha Hres]".
-      iDestruct (IHla with "Hres") as (lv) "(%Hlen & Hres & Hlv)".
-      iDestruct ( opening_closing_resources with "Ha" ) as (va) "[Hres_a Ha]".
-      iExists (va::lv).
-      iFrame.
-      iPureIntro ; cbn ; lia.
-  Qed.
-
-  (* TODO any way to generalize? Or would it be worth re-inlining?? *)
-  (* TODO isn't it JUST open_world_interp_opening_resources + decompose_opening_to_closing_resources ?? *)
+  Lemma StackWorldResources_length (interp : V) (W : WORLD) (C : CmptName) (la : list Addr) (lw : list Word) :
+    StackWorldResources interp W C la lw -∗ ⌜ length la = length lw ⌝.
+  Proof. iIntros "H"; iApply (big_sepL2_length with "H"). Qed.
 
   Lemma open_world_interp_callee_stack (W : WORLD) (C : CmptName) (b_stk e_stk a_stk a_stk4 : Addr)
     ccrel
@@ -232,14 +187,8 @@ Section switcher_helper.
 
     world_interp_open W C (l_callee_stack_frame ++ l_register_save_area) ∗
     (∃ (lv : list Word),
-        ⌜ length lv = length l_callee_stack_frame ⌝
-        ∗ ([∗ list] a ; v ∈ l_callee_stack_frame ; lv, a ↦ₐ v)
-        (* TODO following resources is (only) used by closing_resources_zeros,
-           and in closing_resources_zeros' + close_world_interp_opening_resources,
-           and is (essentially!) generated from open_world_interp_opening_resources...
-           Any ways to makes that look better ??
-         *)
-        ∗ ▷ ([∗ list] a ; v ∈ l_callee_stack_frame ; lv, closing_resources interp W C a v)
+        ([∗ list] a ; v ∈ l_callee_stack_frame ; lv, a ↦ₐ v)
+        ∗ ▷ StackWorldResources interp W C l_callee_stack_frame lv
     )
   .
   Proof.
@@ -269,69 +218,40 @@ Section switcher_helper.
       replace ((a_stk ^+ 2) ^+ 1)%a with (a_stk ^+ 3)%a by solve_addr+Ha_stk4.
       set_solver.
     }
-    iDestruct (decompose_opening_to_closing_resources with "Hres") as "(%&$&$&$)".
   Qed.
 
 
   (* TODO The result matches the excepted shape for E_K *)
-  Lemma closing_resources_zeros (W : WORLD) (C : CmptName) (b e : Addr) (lv : list Word) :
-    let lv' := region_addrs_zeroes b e in
-    length lv = length (finz.seq_between b e) ->
-    Forall (λ y : Word, y = WInt 0) lv' ->
-    ([∗ list] a;v ∈ finz.seq_between b e;lv, closing_resources interp W C a v) -∗
-    ([∗ list] a;v ∈ finz.seq_between b e;lv', closing_resources interp W C a v)
-  .
-    intros lv'.
-    iIntros (Hlen_lv Hlv') "Hres".
-    iAssert (([∗ list] a ∈ finz.seq_between b e, closing_resources interp W C a (WInt 0)))%I
-      with "[Hres]" as "Hres".
-    {
-      iClear "#".
-      clear -Hlen_lv.
-      iStopProof.
-      revert Hlen_lv.
-      generalize dependent lv.
-      generalize (finz.seq_between b e) as la.
-      induction la; iIntros (lv Hlen) "H"; destruct lv as [|v lv]; simplify_eq; cbn; first done.
-      iDestruct "H" as "[Ha H]".
-      iDestruct (closing_resources_zeroed with "Ha") as "$".
-      by iApply (IHla with "H").
-    }
-    rewrite /region_pointsto.
-    iApply big_sepL2_replicate_r; auto.
-    by rewrite finz_seq_between_length.
+  Lemma StackWorldResource_zero (W : WORLD) (C : CmptName) (a : Addr) (v : Word) :
+    StackWorldResource interp W C a v -∗
+    StackWorldResource interp W C a (WInt 0).
+  Proof.
+    iIntros "(%Pa & %pa & $ & HPa & Hmono & $ & ($&#Hzcond&#Hrcond&#Hwcond&%) & $)"; iFrame "#%".
+    specialize (H (W,C,v)).
+    iSplitR "Hmono".
+    + iApply "Hwcond"; iApply interp_int.
+    + rewrite /mono_temporary.
+      destruct ( decide (isWL pa = true ∨ isDL pa = true) )
+      ; iIntros (???) "!>H /="; iApply "Hzcond"; done.
   Qed.
 
-  (* TODO note the slight difference from above: contains a ↦ₐ v *)
-  Lemma closing_resources_zeros' (W : WORLD) (C : CmptName) (b e : Addr) (lv : list Word) :
-    let lv' := region_addrs_zeroes b e in
-    length lv = length (finz.seq_between b e) ->
+    Lemma StackWorldResources_zeros (W : WORLD) (C : CmptName) (la : list Addr) (lv lv': list Word) :
+    length lv = length la ->
+    length lv' = length la ->
     Forall (λ y : Word, y = WInt 0) lv' ->
-    ([∗ list] a;v ∈ finz.seq_between b e;lv, closing_resources interp W C a v) ∗
-    [[b,e]]↦ₐ[[lv']]
-    -∗
-    ([∗ list] a;v ∈ finz.seq_between b e;lv', a ↦ₐ v ∗ closing_resources interp W C a v)
-  .
-    intros lv'.
-    iIntros (Hlen_lv Hlv') "(Hres & Hstk)".
-    rewrite /region_pointsto.
-    iStopProof.
-    assert (length lv' = length (finz.seq_between b e)) as Hlen_lv'.
-    { subst lv'. by rewrite /region_addrs_zeroes length_replicate finz_seq_between_length. }
-    revert Hlen_lv Hlen_lv' Hlv'.
-    generalize dependent lv.
-    generalize dependent lv'.
-    generalize (finz.seq_between b e) as la.
-    induction la; iIntros (lv' lv Hlen' Hlen Hlv') "H"
-    ; destruct lv as [|v lv]; simplify_eq; cbn
-    ; destruct lv' as [|v' lv']; simplify_eq; cbn
-    ; first done.
-    iDestruct "H" as "[ [Hclose Hres] [Ha H] ]"; iFrame.
-    apply Forall_cons in Hlv' ; destruct Hlv' as [-> Hlv'].
-    iDestruct (closing_resources_zeroed with "Hclose") as "$".
-    iApply (IHla with "[Hres H]"); last iFrame; eauto.
+    StackWorldResources interp W C la lv -∗
+    StackWorldResources interp W C la lv'.
+  Proof.
+    move: lv lv'.
+    induction la; iIntros (lv lv' Hlen_lv Hlen_lv' Hzeros) "H"
+    ; destruct lv as [|v lv]; auto
+    ; destruct lv' as [|v' lv']; try done.
+    simplify_eq.
+    apply Forall_cons in Hzeros as [-> Hzeros].
+    iDestruct "H" as "[Ha H]".
+    iSplitL "Ha"; first by iApply StackWorldResource_zero.
+    iApply (IHla lv lv'); eauto.
   Qed.
-
 
   (* TODO ONLY USED RETURN SPEC *)
     Lemma open_world_interp_cframe_gen
@@ -796,6 +716,6 @@ Section switcher_helper.
                "[$Hworld_interp Hrevoked Hstk]") as "Hworld_interp"; last by iFrame.
         rewrite /close_list_resources_gen big_sepL_app.
         iFrame.
-
     Qed.
+
 End switcher_helper.
